![[Pasted image 20230505220800.png]]

$$\overrightarrow{s}=\overrightarrow{a}+\overrightarrow{b}$$

![[Pasted image 20230505221230.png]]
قانون جابجایی:
$$\overrightarrow{a}+\overrightarrow{b}=\overrightarrow{b}+\overrightarrow{a}$$

![[Pasted image 20230505221256.png]]
شرکت پذیری:
$$(\overrightarrow{a}+\overrightarrow{b})+ \overrightarrow{c}=\overrightarrow{a}+(\overrightarrow{b}+\overrightarrow{c})$$

![[Pasted image 20230505221726.png]]
تفریق برداری:
$$\overrightarrow{d}=\overrightarrow{a}-\overrightarrow{b}=\overrightarrow{a}+(-\overrightarrow{b})$$

![[Pasted image 20230505221630.png]]

$$\overrightarrow{b}+(-\overrightarrow{b})=0$$


